proof/refine/ARM_HYP/TcbAcc_R.thy
@@ -562,7 +562,8 @@ lemma setObject_tcb_arch' [wp]:
 
 lemma setObject_tcb_valid_arch' [wp]:
   "\<lbrace>valid_arch_state'\<rbrace> setObject t (v :: tcb) \<lbrace>\<lambda>rv. valid_arch_state'\<rbrace>"
-  by (wp valid_arch_state_lift' setObject_typ_at')
+  apply (wp valid_arch_state_lift' setObject_typ_at')
+  sorry (* valid_arch_state *)
 
 lemma setObject_tcb_refs' [wp]:
   "\<lbrace>\<lambda>s. P (global_refs' s)\<rbrace> setObject t (v::tcb) \<lbrace>\<lambda>rv s. P (global_refs' s)\<rbrace>"
